src/ReactorModel/Execution/Context.lean
@@ -6,6 +6,10 @@ structure Execution.Context (ι) where
   executedRcns : Time.Tag ▸ Finset ι
   nonempty : executedRcns.nonempty
 
+structure Execution.State (ι υ) [Value υ] where
+  rtr : Reactor ι υ
+  ctx : Context ι
+
 namespace Execution.Context
 
 variable {ι υ} [Value υ]
