src/ReactorModel/Execution/Determinism.lean
@@ -15,53 +15,35 @@ theorem ChangeStep.eq_rcns {σ₁ σ₂ : Reactor ι υ} {c : Change ι υ} {g :
   σ₁ -[c, g]→ σ₂ → σ₁.rcns = σ₂.rcns := by
   intro h; cases h <;> simp only <;> (apply Reactor.Update.ne_cmp_and_ne_rtr_eq Cmp.rcn; assumption; all_goals { by_contra; contradiction })
 
-theorem InstExecution.preserves_time {σ₁ σ₂ : Reactor ι υ} {ctx₁ ctx₂ : Context ι} :
-  (σ₁, ctx₁) ⇓ᵢ+ (σ₂, ctx₂) → ctx₁.time = ctx₂.time := by
+theorem InstExecution.preserves_time {s₁ s₂ : State ι υ} :
+  (s₁ ⇓ᵢ+ s₂) → s₁.ctx.time = s₂.ctx.time := by
   intro h
   induction h
   case single h => cases h <;> simp [Context.addCurrentExecuted_same_time]
-  case trans ctx₁ ctx₂ _ h₁₂ h₂₃ hi => 
-    have ht : ctx₁.time = ctx₂.time := by cases h₁₂ <;> simp [Context.addCurrentExecuted_same_time]
+  case trans s₁ s₂ _ h₁₂ h₂₃ hi => 
+    have ht : s₁.ctx.time = s₂.ctx.time := by cases h₁₂ <;> simp [Context.addCurrentExecuted_same_time]
     simp [hi, ht]
 
-theorem InstExecution.preserves_ctx_past_future {σ₁ σ₂ : Reactor ι υ} {ctx₁ ctx₂ : Context ι} (h : (σ₁, ctx₁) ⇓ᵢ+ (σ₂, ctx₂)) :
-  ∀ g, g ≠ ctx₁.time → ctx₁.executedRcns g = ctx₂.executedRcns g := by
-  intro g hg
+theorem InstExecution.preserves_ctx_past_future {s₁ s₂ : State ι υ} :
+  (s₁ ⇓ᵢ+ s₂) → ∀ g, g ≠ s₁.ctx.time → s₁.ctx.executedRcns g = s₂.ctx.executedRcns g := by
+  intro h g hg
   induction h
   case single h => cases h <;> simp [Context.addCurrentExecuted, Finmap.update_ne]
-  case trans ctx₁ ctx₂ ctx₃ he he' hi =>
-    have hc : ctx₁.executedRcns g = ctx₂.executedRcns g := by cases he <;> simp [Context.addCurrentExecuted, Finmap.update_ne]
+  case trans s₁ s₂ _ he _ hi =>
+    have hc : s₁.ctx.executedRcns g = s₂.ctx.executedRcns g := by cases he <;> simp [Context.addCurrentExecuted, Finmap.update_ne]
     rw [InstExecution.preserves_time $ single he] at hg
     simp [hc, hi hg]
 
 -- This theorem is the main theorem about determinism in an instantaneous setting.
 -- Basically, if the same reactions have been executed, then we have the same resulting
 -- reactor.
-theorem InstExecution.deterministic {σ σ₁ σ₂ : Reactor ι υ} {ctx ctx' : Context ι} : 
-  (σ, ctx) ⇓ᵢ+ (σ₁, ctx') → (σ, ctx) ⇓ᵢ+ (σ₂, ctx') → σ₁ = σ₂ := sorry
+theorem InstExecution.deterministic {s s₁ s₂ : State ι υ} : 
+  (s ⇓ᵢ+ s₁) → (s ⇓ᵢ+ s₂) → (s₁.ctx = s₂.ctx) → s₁.rtr = s₂.rtr := sorry
 
-theorem StuckInstExecution.ctx_current_complete {σ₁ σ₂ : Reactor ι υ} {ctx₁ ctx₂ : Context ι} :
-  (σ₁, ctx₁) ⇓ᵢ| (σ₂, ctx₂) → ctx₂.executedRcns ctx₁.time = σ₁.rcns.ids := by
-  intro h
-  have ht : ctx₁.time = ctx₂.time := InstExecution.preserves_time h.exec
-  have hr : σ₁.rcns = σ₂.rcns := sorry
-  rw [ht, hr]
+theorem StuckInstExecution.ctx_current_complete {s₁ s₂ : State ι υ} :
+  (s₁ ⇓ᵢ| s₂) → s₂.ctx.executedRcns s₂.ctx.time = s₂.rtr.rcns.ids := by
   sorry -- This is probably non-trivial.
 
-theorem StuckInstExecution.eq_ctx {σ σ₁ σ₂ : Reactor ι υ} {ctx ctx₁ ctx₂ : Context ι} :
-  (σ, ctx) ⇓ᵢ| (σ₁, ctx₁) → (σ, ctx) ⇓ᵢ| (σ₂, ctx₂) → ctx₁ = ctx₂ := by
-  intro hs₁ hs₂
-  apply Context.ext_iff.mpr; apply Finmap.ext
-  intro g
-  by_cases hg : g = ctx.time
-  case pos => simp [hg, hs₁.ctx_current_complete, hs₂.ctx_current_complete]
-  case neg => simp [←hs₁.exec.preserves_ctx_past_future g hg, hs₂.exec.preserves_ctx_past_future g hg]
-
-theorem StuckInstExecution.convergent {σ σ₁ σ₂ : Reactor ι υ} {ctx ctx₁ ctx₂ : Context ι} :
-  (σ, ctx) ⇓ᵢ| (σ₁, ctx₁) → (σ, ctx) ⇓ᵢ| (σ₂, ctx₂) → σ₁ = σ₂ := by
-  intro hs₁ hs₂
-  rw [←StuckInstExecution.eq_ctx hs₁ hs₂] at hs₂
-  exact InstExecution.deterministic hs₁.exec hs₂.exec
   
 -- The set of reactions can change because of mutations.
 -- However, these changes are deterministic.
@@ -72,30 +54,46 @@ theorem StuckInstExecution.convergent {σ σ₁ σ₂ : Reactor ι υ} {ctx ctx�
 --  sameReactionExecuted ((σ₁, ctx₁) ⇓ᵢ (σ₁', ctx₁')) ((σ₂, ctx₂) ⇓ᵢ (σ₂', ctx₂')) →
 --  sameReactionTopologyChanges ((σ₁, ctx₁) ⇓ᵢ (σ₁', ctx₁')) ((σ₂, ctx₂) ⇓ᵢ (σ₂', ctx₂')) :=
 --  sorry
-lemma inst_convergent_topology {σ σ₁ σ₂ : Reactor ι υ} {ctx ctx₁ ctx₂  : Context ι} :
-    (σ, ctx) ⇓ᵢ| (σ₁, ctx₁) →
-    (σ, ctx) ⇓ᵢ| (σ₂, ctx₂) →
-    σ₁.rcns.ids = σ₂.rcns.ids := by 
-    sorry -- will surely need networkChangeDeterministic (and that should be made to work, too)
 
-theorem Execution.timed_deterministic {σ σ₁ σ₂ : Reactor ι υ} {ctx ctx₁ ctx₂ : Context ι} : 
-  (σ, ctx) ⇓ (σ₁, ctx₁) → (σ, ctx) ⇓ (σ₂, ctx₂) → σ₁ = σ₂ := by
+theorem StuckInstExecution.topology_convergent {s s₁ s₂ : State ι υ} :
+  (s ⇓ᵢ| s₁) → (s ⇓ᵢ| s₂) → s₁.rtr.rcns = s₂.rtr.rcns := 
+  sorry
+
+theorem StuckInstExecution.eq_ctx {s s₁ s₂ : State ι υ} :
+  (s ⇓ᵢ| s₁) → (s ⇓ᵢ| s₂) → s₁.ctx = s₂.ctx := by
+  intro hs₁ hs₂
+  apply Context.ext_iff.mpr; apply Finmap.ext
+  intro g
+  by_cases hg : g = s.ctx.time
+  case pos => 
+    have h₁ := hs₁.ctx_current_complete
+    have h₂ := hs₂.ctx_current_complete
+    simp only [←hs₁.exec.preserves_time, ←hs₂.exec.preserves_time, ←hg] at h₁ h₂
+    simp only [h₁, h₂, StuckInstExecution.topology_convergent hs₁ hs₂]
+  case neg => simp only [←hs₁.exec.preserves_ctx_past_future g hg, hs₂.exec.preserves_ctx_past_future g hg]
+
+theorem StuckInstExecution.convergent {s s₁ s₂ : State ι υ} :
+  (s ⇓ᵢ| s₁) → (s ⇓ᵢ| s₂) → s₁.rtr = s₂.rtr :=
+  λ hs₁ hs₂ => InstExecution.deterministic hs₁.exec hs₂.exec $ StuckInstExecution.eq_ctx hs₁ hs₂
+
+theorem Execution.timed_deterministic {s s₁ s₂ : State ι υ} : 
+  (s ⇓ s₁) → (s ⇓ s₂) → s₁.rtr = s₂.rtr := by
   intro he₁ he₂
   cases he₁ <;> cases he₂
   case instToStuck.instToStuck hs₁ hs₂ => exact StuckInstExecution.convergent hs₁ hs₂
-  case advanceTime.advanceTime h₁ _ _ _ _ _ h₂ => exact Reactor.eqWithClearedPortsUnique h₁ h₂
+  case advanceTime.advanceTime h₁ _ _ _ _ _ _ h₂ => exact Reactor.eqWithClearedPortsUnique h₁ h₂
   -- https://leanprover.zulipchat.com/#narrow/stream/270676-lean4/topic/Collapse.20cases
-  case instToStuck.advanceTime hs _ _ _ _ hr _ => 
+  case instToStuck.advanceTime hs _ _ _ _ _ _ _ => 
     cases hs.exec 
     case single hi =>
       cases hi <;> (
-        have := mt (Finset.ext_iff.mp hr _).mpr <| (by assumption)
+        have := mt (Finset.ext_iff.mp (by assumption) _).mpr <| (by assumption)
         have := Finmap.ids_def'.mpr ⟨_, Eq.symm (by assumption)⟩
         contradiction
       )
     case trans _ hi _ => 
       cases hi <;> (
-        have := mt (Finset.ext_iff.mp hr _).mpr <| (by assumption)
+        have := mt (Finset.ext_iff.mp (by assumption) _).mpr <| (by assumption)
         have := Finmap.ids_def'.mpr ⟨_, Eq.symm (by assumption)⟩
         contradiction
       )
@@ -103,13 +101,13 @@ theorem Execution.timed_deterministic {σ σ₁ σ₂ : Reactor ι υ} {ctx ctx�
     cases hs.exec 
     case single hi =>
       cases hi <;> (
-        have := mt (Finset.ext_iff.mp hr _).mpr <| (by assumption)
+        have := mt (Finset.ext_iff.mp (by assumption) _).mpr <| (by assumption)
         have := Finmap.ids_def'.mpr ⟨_, Eq.symm (by assumption)⟩
         contradiction
       )
     case trans _ hi _ => 
       cases hi <;> (
-        have := mt (Finset.ext_iff.mp hr _).mpr <| (by assumption)
+        have := mt (Finset.ext_iff.mp (by assumption) _).mpr <| (by assumption)
         have := Finmap.ids_def'.mpr ⟨_, Eq.symm (by assumption)⟩
         contradiction
       )
